SSA/Projects/InstCombine/Base.lean
@@ -59,6 +59,14 @@ instance : Goedel Ty where
 toType := fun
   | .bitvec (.concrete w) => Option $ BitVec w
 
+instance (ty : Ty) : Coe ℤ (Goedel.toType ty) where
+  coe z := match ty with
+ | .bitvec (.concrete w) => some <| BitVec.ofInt w z
+
+instance (ty : Ty) : Inhabited (Goedel.toType ty) where
+  default := match ty with
+ | .bitvec (.concrete _) => default
+
 instance : Repr (BitVec n) where
   reprPrec
     | v, n => reprPrec (BitVec.toInt v) n
